wip: parameterizing wp with forking bit

trillium/bi/weakestpre.v
@@ -17,6 +17,21 @@ Proof. split; by repeat intros []. Qed.
 Definition stuckness_to_atomicity (s : stuckness) : atomicity :=
   if s is MaybeStuck then StronglyAtomic else WeaklyAtomic.
 
+(** We now explicitly denote whether the expression under wp is allowed to fork.
+    For all previous developments, CanFork is used. *)
+Inductive forks_bit := CannotFork | CanFork. 
+
+Definition forks_bit_leb (f1 f2 : forks_bit) : bool :=
+  match f1, f2 with
+  | CanFork, CannotFork => false
+  | _, _ => true
+  end.
+#[global] Instance forks_bit_le : SqSubsetEq forks_bit := forks_bit_leb.
+#[global] Instance forks_bit_po : PreOrder forks_bit_le.
+Proof. split; by repeat intros []. Qed.
+
+(* TODO: update the explanation below to accomodate changes from Trillium *)
+
 (** Weakest preconditions [WP e @ s ; E {{ Φ }}] have an additional argument [s]
 of arbitrary type [A], that can be chosen by the one instantiating the [Wp] type
 class. This argument can be used for e.g. the stuckness bit (as in Iris) or
@@ -28,50 +43,61 @@ and [s] to be [NotStuck] or [MaybeStuck].  This will fail to typecheck if [A] is
 not [stuckness].  If we ever want to use the notation [WP e @ E {{ Φ }}] with a
 different [A], the plan is to generalize the notation to use [Inhabited] instead
 to pick a default value depending on [A]. *)
-Class Wp (Λ : language) (PROP A : Type) :=
-  wp : A → coPset -> locale Λ -> expr Λ → (val Λ → PROP) → PROP.
-Arguments wp {_ _ _ _} _ _ _ _%E _%I.
-#[global] Instance: Params (@wp) 8 := {}.
+Class Wp (Λ : language) (PROP A B : Type) :=
+  wp : A → B -> coPset -> locale Λ -> expr Λ → (val Λ → PROP) → PROP.
+Arguments wp {_ _ _ _ _} _ _ _ _%E _%I.
+#[global] Instance: Params (@wp) 9 := {}.
 
 (** Notations for partial weakest preconditions *)
 (** Notations without binder -- only parsing because they overlap with the
 notations with binder. *)
 
-
-Notation "'WP' e @ s ; tid ; E {{ Φ } }" := (wp s E tid e%E Φ)
+(** Allow forking by default; to prohibit it, the "most detailed" notation is needed *)
+Notation "'WP' e @ f ; s ; tid ; E {{ Φ } }" := (wp s f E tid e%E Φ)
   (at level 20, e, Φ at level 200, only parsing) : bi_scope.
-Notation "'WP' e @ tid ; E {{ Φ } }" := (wp NotStuck E tid e%E Φ)
+Notation "'WP' e @ s ; tid ; E {{ Φ } }" := (wp s CanFork E tid e%E Φ)
   (at level 20, e, Φ at level 200, only parsing) : bi_scope.
-Notation "'WP' e @ tid ; E ? {{ Φ } }" := (wp MaybeStuck E tid e%E Φ)
+Notation "'WP' e @ tid ; E {{ Φ } }" := (wp NotStuck CanFork E tid e%E Φ)
   (at level 20, e, Φ at level 200, only parsing) : bi_scope.
-Notation "'WP' e @ tid {{ Φ } }" := (wp NotStuck ⊤ tid e%E Φ)
+Notation "'WP' e @ tid ; E ? {{ Φ } }" := (wp MaybeStuck CanFork E tid e%E Φ)
   (at level 20, e, Φ at level 200, only parsing) : bi_scope.
-Notation "'WP' e @ tid ? {{ Φ } }" := (wp MaybeStuck ⊤ tid e%E Φ)
+Notation "'WP' e @ tid {{ Φ } }" := (wp NotStuck CanFork ⊤ tid e%E Φ)
+  (at level 20, e, Φ at level 200, only parsing) : bi_scope.
+Notation "'WP' e @ tid ? {{ Φ } }" := (wp MaybeStuck CanFork ⊤ tid e%E Φ)
   (at level 20, e, Φ at level 200, only parsing) : bi_scope.
 
 (** Notations with binder.  The indentation for the inner format block is chosen
 such that *if* one has a single-character mask (e.g. [E]), the second line
 should align with the binder(s) on the first line. *)
-Notation "'WP' e @ s ; tid ; E {{ v , Q } }" := (wp s E tid e%E (λ v, Q))
+Notation "'WP' e @ f ; s ; tid ; E {{ v , Q } }" := (wp s f E tid e%E (λ v, Q))
+  (at level 20, e, Q at level 200,
+   format "'[' 'WP'  e  '/' '[          ' @  f ;  s ;  tid ;  E  {{  v ,  Q  } } ']' ']'") : bi_scope.
+Notation "'WP' e @ s ; tid ; E {{ v , Q } }" := (wp s CanFork E tid e%E (λ v, Q))
   (at level 20, e, Q at level 200,
    format "'[' 'WP'  e  '/' '[          ' @  s ;  tid ;  E  {{  v ,  Q  } } ']' ']'") : bi_scope.
-Notation "'WP' e @ tid ; E {{ v , Q } }" := (wp NotStuck E tid e%E (λ v, Q))
+Notation "'WP' e @ tid ; E {{ v , Q } }" := (wp NotStuck CanFork E tid e%E (λ v, Q))
   (at level 20, e, Q at level 200,
    format "'[' 'WP'  e  '/' '[       ' @  tid ;  E  {{  v ,  Q  } } ']' ']'") : bi_scope.
-Notation "'WP' e @ tid ; E ? {{ v , Q } }" := (wp MaybeStuck E tid e%E (λ v, Q))
+Notation "'WP' e @ tid ; E ? {{ v , Q } }" := (wp MaybeStuck CanFork E tid e%E (λ v, Q))
   (at level 20, e, Q at level 200,
    format "'[' 'WP'  e  '/' '[        ' @  tid ;  E  ? {{  v ,  Q  } } ']' ']'") : bi_scope.
-Notation "'WP' e @ tid {{ v , Q } }" := (wp NotStuck ⊤ tid e%E (λ v, Q))
+Notation "'WP' e @ tid {{ v , Q } }" := (wp NotStuck CanFork ⊤ tid e%E (λ v, Q))
   (at level 20, e, Q at level 200,
    format "'[' 'WP'  e  @ tid  '/' '[   ' {{  v ,  Q  } } ']' ']'") : bi_scope.
-Notation "'WP' e @ tid ? {{ v , Q } }" := (wp MaybeStuck ⊤ tid e%E (λ v, Q))
+Notation "'WP' e @ tid ? {{ v , Q } }" := (wp MaybeStuck CanFork ⊤ tid e%E (λ v, Q))
   (at level 20, e, Q at level 200,
    format "'[' 'WP'  e  @ tid  '/' '[    ' ? {{  v ,  Q  } } ']' ']'") : bi_scope.
 
 (* Texan triples *)
+(* TODO: order of parameters is different from WP; fix it? *)
+Notation "'{{{' P } } } e @ tid ; f ; s ; E {{{ x .. y , 'RET' pat ; Q } } }" :=
+  (□ ∀ Φ,
+      P -∗ ▷ (∀ x, .. (∀ y, Q -∗ Φ pat%V) .. ) -∗ WP e @ f; s; tid; E {{ Φ }})%I
+    (at level 20, x closed binder, y closed binder,
+     format "'[hv' {{{  P  } } }  '/  ' e  '/' @ tid ;  f ; s ;  E  {{{  x  ..  y ,  RET  pat ;  Q  } } } ']'") : bi_scope.
 Notation "'{{{' P } } } e @ tid ; s ; E {{{ x .. y , 'RET' pat ; Q } } }" :=
   (□ ∀ Φ,
-      P -∗ ▷ (∀ x, .. (∀ y, Q -∗ Φ pat%V) .. ) -∗ WP e @ tid ; s; E {{ Φ }})%I
+      P -∗ ▷ (∀ x, .. (∀ y, Q -∗ Φ pat%V) .. ) -∗ WP e @ s ; tid; E {{ Φ }})%I
     (at level 20, x closed binder, y closed binder,
      format "'[hv' {{{  P  } } }  '/  ' e  '/' @ tid ;  s ;  E  {{{  x  ..  y ,  RET  pat ;  Q  } } } ']'") : bi_scope.
 Notation "'{{{' P } } } e @ tid ; E {{{ x .. y , 'RET' pat ; Q } } }" :=
@@ -95,6 +121,10 @@ Notation "'{{{' P } } } e @ tid ? {{{ x .. y , 'RET' pat ; Q } } }" :=
     (at level 20, x closed binder, y closed binder,
      format "'[hv' {{{  P  } } }  '/  ' e  @ tid '/' ? {{{  x  ..  y ,   RET  pat ;  Q  } } } ']'") : bi_scope.
 
+Notation "'{{{' P } } } e @ f ; s ; tid ; E {{{ 'RET' pat ; Q } } }" :=
+  (□ ∀ Φ, P -∗ ▷ (Q -∗ Φ pat%V) -∗ WP e @ f; s; tid ; E {{ Φ }})%I
+    (at level 20,
+     format "'[hv' {{{  P  } } }  '/  ' e  '/' @ f ; s ; tid  ; E  {{{  RET  pat ;  Q  } } } ']'") : bi_scope.
 Notation "'{{{' P } } } e @ s ; tid ; E {{{ 'RET' pat ; Q } } }" :=
   (□ ∀ Φ, P -∗ ▷ (Q -∗ Φ pat%V) -∗ WP e @ s; tid ; E {{ Φ }})%I
     (at level 20,
@@ -117,6 +147,8 @@ Notation "'{{{' P } } } e @ tid ? {{{ 'RET' pat ; Q } } }" :=
      format "'[hv' {{{  P  } } }  '/  ' e @ tid '/' ? {{{  RET  pat ;  Q  } } } ']'") : bi_scope.
 
 (** Aliases for stdpp scope -- they inherit the levels and format from above. *)
+Notation "'{{{' P } } } e @ f ; s ; tid ; E {{{ x .. y , 'RET' pat ; Q } } }" :=
+  (∀ Φ, P -∗ ▷ (∀ x, .. (∀ y, Q -∗ Φ pat%V) .. ) -∗ WP e @ f; s; tid ; E {{ Φ }}) : stdpp_scope.
 Notation "'{{{' P } } } e @ s ; tid ; E {{{ x .. y , 'RET' pat ; Q } } }" :=
   (∀ Φ, P -∗ ▷ (∀ x, .. (∀ y, Q -∗ Φ pat%V) .. ) -∗ WP e @ s; tid ; E {{ Φ }}) : stdpp_scope.
 Notation "'{{{' P } } } e @ tid ; E {{{ x .. y , 'RET' pat ; Q } } }" :=
@@ -127,6 +159,8 @@ Notation "'{{{' P } } } e @ tid {{{ x .. y , 'RET' pat ; Q } } }" :=
   (∀ Φ, P -∗ ▷ (∀ x, .. (∀ y, Q -∗ Φ pat%V) .. ) -∗ WP e @ tid {{ Φ }}) : stdpp_scope.
 Notation "'{{{' P } } } e @ tid ? {{{ x .. y , 'RET' pat ; Q } } }" :=
   (∀ Φ, P -∗ ▷ (∀ x, .. (∀ y, Q -∗ Φ pat%V) .. ) -∗ WP e @ tid ?{{ Φ }}) : stdpp_scope.
+Notation "'{{{' P } } } e @ f ; s ; tid ; E {{{ 'RET' pat ; Q } } }" :=
+  (∀ Φ, P -∗ ▷ (Q -∗ Φ pat%V) -∗ WP e @ f; s; tid; E {{ Φ }}) : stdpp_scope.
 Notation "'{{{' P } } } e @ s ; tid ; E {{{ 'RET' pat ; Q } } }" :=
   (∀ Φ, P -∗ ▷ (Q -∗ Φ pat%V) -∗ WP e @ s; tid; E {{ Φ }}) : stdpp_scope.
 Notation "'{{{' P } } } e @ tid ; E {{{ 'RET' pat ; Q } } }" :=
